src/tls/ECGroup.fst
@@ -82,20 +82,6 @@ let parse_curve b =
        | _                   -> None)
     | _ -> None)
 
-val curve_id: group -> Tot (lbytes 2)
-let curve_id g =
-  let open Format.NamedGroup in
-  let r = namedGroup_serializer32 ( // <- curve_id == namedGroup_serializer
-    match g with
-    | ECC_P256   -> SECP256R1
-    | ECC_P384   -> SECP384R1
-    | ECC_P521   -> SECP521R1
-    | ECC_X25519 -> X25519
-    | ECC_X448   -> X448) in
-  assume (length r = 2);
-  r
-
-#reset-options "--using_facts_from '* -LowParse'"
 let parse_point g b =
   // parser for flat bytes or uncompressedPointPepresentation
   match g with
@@ -142,6 +128,7 @@ let parse_partial payload =
 
 open FStar.Mul
 
+#reset-options "--using_facts_from '* -LowParse'"
 (* Assumes uncompressed point format for now (04||ecx||ecy) *)
 let serialize_point #g s =
   match g with
@@ -165,51 +152,24 @@ let serialize_point #g s =
     assume (length x = 2 * (ec_bytelen g) + 1);
     x
 
+let curve_id g : Tot (lbytes 2) =
+  let open Format.NamedGroup in
+  let r = namedGroup_serializer32 ( // <- curve_id == namedGroup_serializer
+    match g with
+    | ECC_P256   -> SECP256R1
+    | ECC_P384   -> SECP384R1
+    | ECC_P521   -> SECP521R1
+    | ECC_X25519 -> X25519
+    | ECC_X448   -> X448) in
+  assume (length r = 2);
+  r
+
 let serialize #g ecdh_Y =
   // Similar to parse_partial, we should rewrite this using serializer combinators
   let ty = abyte 3z in
   let id = curve_id g in
   let e = serialize_point ecdh_Y in
   lemma_repr_bytes_values (FStar.Bytes.length e);
+  assert (repr_bytes (length e) <= 1);
   let ve = vlbytes 1 e in
   ty @| id @| ve
-#reset-options
-
-(* KB: older more general code below
-let getParams (c : ec_curve) : ec_params =
-    let rawcurve : ec_prime = match c with
-    | ECC_P256 ->
-        {
-            ecp_prime = "115792089210356248762697446949407573530086143415290314195533631308867097853951";
-            ecp_order = "115792089210356248762697446949407573529996955224135760342422259061068512044369";
-            ecp_a = "115792089210356248762697446949407573530086143415290314195533631308867097853948"; // p-3
-            ecp_b = "5ac635d8aa3a93e7b3ebbd55769886bc651d06b0cc53b0f63bce3c3e27d2604b";
-            ecp_gx = "6b17d1f2e12c4247f8bce6e563a440f277037d812deb33a0f4a13945d898c296";
-            ecp_gy = "4fe342e2fe1a7f9b8ee7eb4a7c0f9e162bce33576b315ececbb6406837bf51f5";
-            ecp_bytelen = 32;
-            ecp_id = twobytes (0z, 23z);
-        }
-    | ECC_P384 ->
-        {
-            ecp_prime = "39402006196394479212279040100143613805079739270465446667948293404245721771496870329047266088258938001861606973112319";
-            ecp_order = "39402006196394479212279040100143613805079739270465446667946905279627659399113263569398956308152294913554433653942643";
-            ecp_a = "39402006196394479212279040100143613805079739270465446667948293404245721771496870329047266088258938001861606973112316"; // p-3
-            ecp_b = "b3312fa7e23ee7e4988e056be3f82d19181d9c6efe8141120314088f5013875ac656398d8a2ed19d2a85c8edd3ec2aef";
-            ecp_gx = "aa87ca22be8b05378eb1c71ef320ad746e1d3b628ba79b9859f741e082542a385502f25dbf55296c3a545e3872760ab7";
-            ecp_gy = "3617de4a96262c6f5d9e98bf9292dc29f8f41dbd289a147ce9da3113b5f0b8c00a60b1ce1d7e819d7a431d7c90ea0e5f";
-            ecp_bytelen = 48;
-            ecp_id = twobytes (0z, 24z);
-        }
-    | ECC_P521 ->
-        {
-            ecp_prime = "6864797660130609714981900799081393217269435300143305409394463459185543183397656052122559640661454554977296311391480858037121987999716643812574028291115057151";
-            ecp_order = "6864797660130609714981900799081393217269435300143305409394463459185543183397655394245057746333217197532963996371363321113864768612440380340372808892707005449";
-            ecp_a = "6864797660130609714981900799081393217269435300143305409394463459185543183397656052122559640661454554977296311391480858037121987999716643812574028291115057148"; // p-3
-            ecp_b = "051953eb9618e1c9a1f929a21a0b68540eea2da725b99b315f3b8b489918ef109e156193951ec7e937b1652c0bd3bb1bf073573df883d2c34f1ef451fd46b503f00";
-            ecp_gx = "0c6858e06b70404e9cd9e3ecb662395b4429c648139053fb521f828af606b4d3dbaa14b5e77efe75928fe1dc127a2ffa8de3348b3c1856a429bf97e7e31c2e5bd66";
-            ecp_gy = "11839296a789a3bc0045c8a5fb42c7d1bd998f54449579b446817afbd17273e662c97ee72995ef42640c550b9013fad0761353c7086a272c24088be94769fd16650";
-            ecp_bytelen = 66;
-            ecp_id = twobytes (0z, 25z);
-        }
-    in { curve = EC_PRIME rawcurve; point_compression = false; }
-*)
